verif

ModularEngine/src/LogicEngine.FStar/interp.fst
@@ -3,10 +3,14 @@ open TypeHeaders
 open Types
 open Util
 open Marshall
+open State
 
 type substrate
 type vars = list var
 type substitutions = list substitution
+
+val me : principal 
+let me = Crypto.lookup_my_credentials ()
 
 type condition =
   | If   : polyterm -> condition
@@ -22,18 +26,68 @@ type action =
 
 type actions = list action
 
+type infon = polyterm
+type communication = i:infon{Net.Received i}
+type communications = list communication
+
+(* -------------------------------------------------------------------------------- *)
+(* Spec: Validity of condition(s) *)
+(* -------------------------------------------------------------------------------- *)
+logic function CondSubst : condition -> substitution -> condition
+assume forall (i:infon). (CondSubst (If i) s) = (If (PolySubst i s))
+assume forall (i:infon). (CondSubst (Upon i) s) = (Upon (PolySubst i s))
+
+logic function ActionSubst : action -> substitution -> action
+assume forall (i:infon). (ActionSubst (Learn i) s) = (Learn (PolySubst i s))
+assume forall (i:infon). (ActionSubst (Drop i) s) = (Drop (PolySubst i s))
+assume forall (p:term) (i:infon). (ActionSubst (Fwd p i) s) = (Fwd (Subst p s) (PolySubst i s))
+assume forall (p:term) (i:infon). (ActionSubst (Send p i) s) = (Send (Subst p s) (PolySubst i s))
+
+type HoldsOne :: vars => condition => substitution => E
+assume forall (xs:vars) (i:infon) (subst:substitution) (s:substrate) (k:infostrate). 
+         ((Includes xs (Domain subst)) && 
+          (Includes xs (FreeVars i)) &&
+          (polyentails s k [] (PolySubst i subst)))
+      => HoldsOne xs (If i) subst
+assume forall (xs:vars) (i:infon) (subst:substitution) (c:communication). 
+         ((Includes xs (Domain subst)) &&
+          (Includes xs (FreeVars i)) &&
+          (c=(PolySubst subst i)))
+      => HoldsOne xs (Upon i) subst
+
+type HoldsMany :: substitution => vars => list condition => substitution => E
+assume forall (s:substitution) (xs:vars).
+          (Includes (Domain s) xs) && (Includes xs (Domain s))
+          =>  HoldsMany s xs [] s
+assume forall (s1:substitution) (xs:vars) (c:condition) (s1':substitution) 
+              (cs:conditions) (s2:substitution). 
+          (HoldsOne xs (CondSubst c s1) s1') && 
+          (HoldsMany s1' xs cs s2)
+          => HoldsMany s1 xs cs s2
+          
+type Holds :: _ = fun (xs:vars) (cs:list condition) (s:substitution) => (HoldsMany EmptySubst xs cs s)
+
+(* -------------------------------------------------------------------------------- *)
+(* Spec: Enabled actions *)
+(* -------------------------------------------------------------------------------- *)
+type Enabled :: action => E
+assume forall (i:infon). (Enabled (Learn i)) => Knows i
+assume forall (p:term) (i:infon).(Enabled (Send p i)) => SaysTo me p i
+
 type rule =
-  | Rule : vars -> conditions -> actions -> rule
+  | Rule : xs:vars 
+        -> cs:conditions 
+        -> acts:actions{forall (a:action) (subst:substitution). In a acts && Holds xs cs subst => (Enabled (ActionSubst a subst))}
+        -> rule
 
 type rules = list rule
-type infon = polyterm
-type communications = list infon
 
 (* ================= Wrapping external functions ===================== *)
-(* val me : principal *)
-let me = Crypto.lookup_my_credentials ()
 
-(* val derive: u:vars -> goal:infon -> s0:substitution -> list substitution *)
+val derive:  u:vars
+          -> goal:infon
+          -> s0:substitution
+          -> list (s:substitution{Holds u (CondSubst (If goal) s0) s})
 let derive u goal s0 = 
   let s = State.getSubstrate () in
   let k = State.getInfostrate () in 
@@ -48,24 +102,24 @@ let derive u goal s0 =
              | Some ((s, pf)) ->  [s])
 
 (* ================= Process state and messaging ===================== *)
+val comms : ref (list communication)
 let comms = ref []
 
 let get_communications _unit = 
   let message = Net.receive () in
-  let infons = Marshall.parse message in 
-    comms := append infons (!comms)
+  let infon = Marshall.parse message in 
+    comms := infon::(!comms)
 
-(* drop infons in co that are the same as i *)
+val dropCommunications: i:infon{Enabled (Drop i)} -> unit
 let dropCommunications i = 
   let changed, comms' = 
     fold_right (fun j (changed, out) -> 
-                  if i=j then (true, out) 
+                  if (i:infon)=j then (true, out) 
                   else (changed, j::out)) (!comms) (false, []) in 
     (comms := comms');
     changed
 
 let outbuffer = ref []
-
 let clear_out_buffer () = outbuffer := []
 
 let dispatch p m = 
@@ -76,30 +130,33 @@ let dispatch p m =
      (Net.send p (Marshall.msg2bytes m));
      true)
 
-(* val fwd : principal -> infon -> bool *)
+val fwd: p:principal -> i:infon{Enabled (Fwd (Const (PrincipalConstant p)) i)} -> bool 
 let fwd p i = 
   let m = Forwarded ({msg_from=me;
                       msg_to=p;
                       msg_payload=i}) in 
     dispatch p m 
   
-(* val send : principal -> infon -> bool *)
+val send : p:principal -> i:infon{Enabled (Send (Const (PrincipalConstant p)) i)} -> bool 
 let send p i = 
-  let m = Justified ({msg_from=me;
-                      msg_to=p;
-                      msg_payload=i}) in 
+  let m = Justified (me, p, i) in 
     dispatch p m 
                                
 (* ========================== Rule engine ==================== *)
-(* val matchComm : comm:infon -> xs:vars -> pat:infon -> substitution -> substitutions  *)
+val matchComm : comm:communication 
+             -> xs:vars -> pat:infon 
+             -> s0:substitution 
+             -> list (s1:substitution{HoldsOne xs (Upon (PolySubst s0 pat))})
 let matchComm comm xs pat s = 
   match Unify.unify_poly s [] xs comm (Subst.polysubst pat s) with 
     | None -> []
-    | Some s1 -> [(s1:substitution)]
-    
+    | Some s1 -> [s1]
+
 let matchComms xs pat s = collect (fun comm -> matchComm comm xs pat s) (!comms)
   
-(* val substAction: substitutions -> action -> actions *)
+val substAction: substs:substitutions 
+              -> a:action 
+              -> acts:actions{Zip (fun subst act => act=(ActionSubst a subst)) substs acts}
 let substAction substs a =
   match a with
     | Learn i -> map (fun s -> Learn (Subst.polysubst i s)) substs
@@ -107,28 +164,29 @@ let substAction substs a =
     | Fwd p i -> map (fun s -> Fwd (Subst.subst p s) (Subst.polysubst i s)) substs
     | Send p i -> map (fun s -> Send (Subst.subst p s) (Subst.polysubst i s)) substs
 
-(* val evalCond: vars -> substitutions -> condition -> substitutions  *)
+val evalCond: xs:vars -> s1:substitutions -> c:condition -> list (s:substition{})
 let evalCond xs sl c = match c with 
   | If i -> collect (fun s -> derive xs (Subst.polysubst i s) s) sl
   | Upon i -> collect (fun s -> matchComms xs (Subst.polysubst i s) s) sl
-      
+
+val evalConds: xs:vars -> cs:conditions -> list (s:substitution{Holds xs cs s})      
 let evalConds xs cs = fold_left (evalCond xs) [(Subst.emptySubst())] cs
 
-(* val holdsOne : rule -> actions *)
-let holdsOne r = match r with 
+val enabledActions : r:rule -> list (a:action{Enabled a})
+let enabledActions r = match r with 
   | Rule xs cs acts ->  collect (substAction (evalConds xs cs)) acts
-let holds rs = collect holdsOne rs
 
+val allEnabledActions : rs:list rule -> list (a:action{Enabled a})
+let allEnabledActions rs = collect holdsOne rs
+
+val asPrincipal: p:term -> q:principal{p=(Const (PrincipalConstant q))}
 let asPrincipal = function 
   | Const (PrincipalConstant p) -> p
   | _ -> raise "Unexpected type"
 
-(* val applyAction: bool -> action -> bool  *)
+val applyAction: b:bool -> a:action{Enabled a} -> bool 
 let applyAction b a =  match a with 
-  | Learn i -> 
-      (assume (State.Valid i)); (* TODO: remove this. *)
-      State.addToInfostrate i;
-      true
+  | Learn i -> State.addToInfostrate i; true
   | Drop i -> dropCommunications i 
   | Fwd p i -> fwd (asPrincipal p) i
   | Send p i -> send (asPrincipal p) i
