ModularEngine/src/LogicEngine.FStar/marshall.fst
@@ -2,16 +2,22 @@ module Marshall
 open TypeHeaders
 open Types
 
-type message = {msg_from:principal;
-                msg_to: principal;
-                msg_payload: polyterm}
+type message :: _ =  fun ('P::principal => principal => polyterm => E) => 
+    ((pfrom:principal *
+        pto:principal *
+          i:polyterm{'P pfrom pto i}))
+
+type SaysTo :: principal => principal => polyterm => E
+type trivial :: _ = (fun (p:principal) (q:principal) (i:polyterm) => True)
+
 type msg = 
-  | Justified : message -> msg
-  | Forwarded : message -> msg
+  | Forwarded : message trivial -> msg
+  | Justified : message SaysTo -> msg
+
 
 val polyterm2bytes : polyterm -> bytes
 val bytes2polyterm : bytes -> polyterm
-val parse: bytes -> list polyterm
+val parse: b:bytes -> p:polyterm{Received b => Received p}
 val concat : list bytes -> bytes
 val unconcat: bytes -> list bytes
 
