ModularEngine/src/LogicEngine.FStar/net.fst
@@ -2,5 +2,8 @@ module Net
 open TypeHeaders
 open Types
 
-val receive: unit -> bytes
+type Received :: 'a::* => 'a => E
+assume forall (x:'a) (l:list 'a). In x l && Received l => Received x
+
+val receive: unit -> b:bytes{Received b}
 val send: principal -> bytes -> unit
